casestudy/README.md
@@ -1,4 +1,6 @@
 # Secure implementation of 64-bit modulo
 
+Implementation is in `../compiler/examples/mod_patch.jazz`
 
-
+Security proof (constant-time in a model in which division/modulo leaks the size of the dividend and the value of the modulus) in `modulo_ct_proof.ec`, lemma `l2`.
+It assumes that the modulus (second argument) is public and non-zero.
